Add NO_MAIN_CALLS and FUNC_NAME to match_states

src/hls/HTLgenproof.v
@@ -145,14 +145,14 @@ Inductive stack_base_sp : list RTL.stackframe -> Values.block -> Prop :=
                     blk'.
 Hint Constructors stack_base_sp : htlproof.
 
-Inductive match_frames (ge : RTL.genv) (current_id : HTL.ident) (mem : Memory.mem)
+Inductive match_frames (prog : RTL.program) (current_id : HTL.ident) (mem : Memory.mem)
   : (list RTL.stackframe) -> (list HTL.stackframe) -> Prop :=
 | match_frames_nil :
-    match_frames ge current_id mem nil nil
+    match_frames prog current_id mem nil nil
 | match_frames_cons :
     forall dst f sp blk rs mid m pc st asr asa rtl_tl htl_tl ret rst fin
       (MASSOC : match_assocmaps f rs asr)
-      (TF : tr_module ge f m)
+      (TF : tr_module (Genv.globalenv prog) f m)
       (MARR : match_arrs m f sp mem asa)
       (SP_VALID : sp_valid sp)
       (SP_BASE : nil_stack_base_sp rtl_tl sp blk \/ stack_base_sp rtl_tl blk)
@@ -162,22 +162,24 @@ Inductive match_frames (ge : RTL.genv) (current_id : HTL.ident) (mem : Memory.me
       (CONST : match_constants m asr)
       (EXTERN_CALLER : has_externctrl m current_id ret rst fin)
       (MEXTERNCTRL : match_externctrl m asr)
+      (NO_MAIN_CALLS : (mid = (AST.prog_main prog) -> rtl_tl = nil))
+      (FUNC_NAME : HTL.find_func (Genv.globalenv prog) mid = Some (AST.Internal f))
       (JOIN_CTRL : (HTL.mod_controllogic m)!st = Some (state_wait (HTL.mod_st m) fin pc))
       (JOIN_DATA : (HTL.mod_datapath m)!st = Some (join fin rst ret dst))
-      (TAILS : match_frames ge mid mem rtl_tl htl_tl)
+      (TAILS : match_frames prog mid mem rtl_tl htl_tl)
       (DST : Ple dst (RTL.max_reg_function f))
       (PC : (Z.pos pc <= Int.max_unsigned)),
-      match_frames ge current_id mem
+      match_frames prog current_id mem
                    ((RTL.Stackframe     dst f sp pc rs     ) :: rtl_tl)
                    ((HTL.Stackframe mid     m    st asr asa) :: htl_tl).
 Hint Constructors match_frames : htlproof.
 
-Inductive match_states (ge : RTL.genv) : RTL.state -> HTL.state -> Prop :=
+Inductive match_states (prog : RTL.program) : RTL.state -> HTL.state -> Prop :=
 | match_state : forall asa asr rtl_stk f sp blk rs mem mid m st htl_stk
     (MASSOC : match_assocmaps f rs asr)
-    (TF : tr_module ge f m)
+    (TF : tr_module (Genv.globalenv prog) f m)
     (WF : state_st_wf m (HTL.State htl_stk mid m st asr asa))
-    (MF : match_frames ge mid mem rtl_stk htl_stk)
+    (MF : match_frames prog mid mem rtl_stk htl_stk)
     (MARR : match_arrs m f sp mem asa)
     (SP_VALID : sp_valid sp)
     (SP_BASE : nil_stack_base_sp rtl_stk sp blk \/ stack_base_sp rtl_stk blk)
@@ -185,28 +187,32 @@ Inductive match_states (ge : RTL.genv) : RTL.state -> HTL.state -> Prop :=
     (ASBP : arr_stack_based_pointers blk mem (f.(RTL.fn_stacksize)) sp)
     (BOUNDS : stack_bounds sp (f.(RTL.fn_stacksize)) mem)
     (CONST : match_constants m asr)
-    (MEXTERNCTRL : match_externctrl m asr),
-    match_states ge
+    (MEXTERNCTRL : match_externctrl m asr)
+    (NO_MAIN_CALLS : (mid = (AST.prog_main prog) -> rtl_stk = nil))
+    (FUNC_NAME : HTL.find_func (Genv.globalenv prog) mid = Some (AST.Internal f)),
+    match_states prog
                  (RTL.State rtl_stk     f sp st rs      mem)
                  (HTL.State htl_stk mid m    st asr asa    )
 | match_returnstate :
     forall v v' rtl_stk htl_stk mem mid sp blk
-      (MF : match_frames ge mid mem rtl_stk htl_stk)
+      (MF : match_frames prog mid mem rtl_stk htl_stk)
       (SP_BASE : nil_stack_base_sp rtl_stk sp blk \/ stack_base_sp rtl_stk blk)
-      (RV_BASED : stack_based v blk)
+      (RV_BASED : rtl_stk = nil \/ stack_based v blk)
       (MV : val_value_lessdef v v'),
-      match_states ge
+      match_states prog
                    (RTL.Returnstate rtl_stk     v  mem)
                    (HTL.Returnstate htl_stk mid v'    )
 | match_call :
     forall f m rtl_args htl_args mid mem rtl_stk htl_stk sp blk
-    (TF : tr_module ge f m)
-    (MF : match_frames ge mid mem rtl_stk htl_stk)
+    (TF : tr_module (Genv.globalenv prog) f m)
+    (MF : match_frames prog mid mem rtl_stk htl_stk)
     (SP_BASE : nil_stack_base_sp rtl_stk sp blk \/ stack_base_sp rtl_stk blk)
     (INIT_CALL_NO_ARGS : rtl_stk = nil -> rtl_args = nil)
     (ARGS_BASED : Forall (fun a => stack_based a blk) rtl_args)
-    (MARGS : list_forall2 val_value_lessdef rtl_args htl_args),
-      match_states ge
+    (MARGS : list_forall2 val_value_lessdef rtl_args htl_args)
+    (NO_MAIN_CALLS : (mid = (AST.prog_main prog) -> rtl_stk = nil))
+    (FUNC_NAME : HTL.find_func (Genv.globalenv prog) mid = Some (AST.Internal f)),
+      match_states prog
                    (RTL.Callstate rtl_stk     (AST.Internal f) rtl_args mem)
                    (HTL.Callstate htl_stk mid m                htl_args).
 Hint Constructors match_states : htlproof.
@@ -214,7 +220,8 @@ Hint Constructors match_states : htlproof.
 Definition match_prog (p: RTL.program) (tp: HTL.program) :=
   Linking.match_program (fun cu f tf => transl_fundef p f = Errors.OK tf) eq p tp /\
   main_is_internal p = true /\
-  only_main_has_stack p.
+  main_not_called p /\
+  only_main_has_ainstack p.
 
 Instance TransfHTLLink (tr_fun: RTL.program -> Errors.res HTL.program):
   TransfLink (fun (p1: RTL.program) (p2: HTL.program) => match_prog p1 p2).
@@ -231,7 +238,9 @@ Proof.
   simplify.
 
   subst.
-  rewrite H5 in *.
+  match goal with
+  | [H : (AST.prog_main _) = (AST.prog_main _) |- _ ] => rewrite H in *; clear H
+  end.
   specialize (H (AST.prog_main p2)).
 
   exploit H.
@@ -256,9 +265,11 @@ Lemma transf_program_match:
 Proof.
   intros. unfold transl_program in H.
   destruct (main_is_internal p) eqn:?; try discriminate.
-  unfold match_prog. split.
-  apply Linking.match_transform_partial_program; auto.
-  assumption.
+  destruct (only_main_has_ainstack_dec p); try discriminate.
+  destruct (main_not_called_dec p); try discriminate.
+  unfold match_prog.
+  crush.
+  apply Linking.match_transform_partial_program. assumption.
 Qed.
 
 Lemma regs_lessdef_empty : forall f, match_assocmaps f (Registers.Regmap.init Values.Vundef) empty_assocmap.
@@ -564,22 +575,22 @@ Section CORRECTNESS.
       corollaries of [ only_main_stores ]
    *)
   Axiom only_main_stores : forall rtl_stk f sp pc pc' rs mem htl_stk mid m asr asa a b c d,
-      match_states ge (RTL.State rtl_stk f sp pc rs mem) (HTL.State htl_stk mid m pc asr asa) ->
+      match_states prog (RTL.State rtl_stk f sp pc rs mem) (HTL.State htl_stk mid m pc asr asa) ->
       (RTL.fn_code f) ! pc = Some (RTL.Istore a b c d pc') ->
       (rtl_stk = nil /\ htl_stk = nil).
 
   Axiom no_stack_functions : forall f sp rs mem st rtl_stk S,
-      match_states ge (RTL.State rtl_stk f sp st rs mem) S ->
+      match_states prog (RTL.State rtl_stk f sp st rs mem) S ->
       (RTL.fn_stacksize f) = 0 \/ rtl_stk = nil.
 
   Axiom no_stack_calls : forall f mem args rtl_stk S,
-      match_states ge (RTL.Callstate rtl_stk (AST.Internal f) args mem) S ->
+      match_states prog (RTL.Callstate rtl_stk (AST.Internal f) args mem) S ->
       (RTL.fn_stacksize f) = 0 \/ rtl_stk = nil.
 
   Lemma mem_free_zero_match_frames : forall rtl_stk htl_stk mem mem' blk id,
       Mem.free mem blk 0 0 = Some mem' ->
-      match_frames ge id mem rtl_stk htl_stk ->
-      match_frames ge id mem' rtl_stk htl_stk.
+      match_frames prog id mem rtl_stk htl_stk ->
+      match_frames prog id mem' rtl_stk htl_stk.
   Proof.
     Lemma mem_free_match_arrs : forall m f sp blk mem mem' asa,
       Mem.free mem blk 0 0 = Some mem' ->
@@ -625,10 +636,10 @@ Section CORRECTNESS.
     induction rtl_stk; intros * Hmem Hstk; inv Hstk; eauto 6 with htlproof.
   Qed.
 
-  Lemma mem_alloc_zero_match_frames : forall rtl_stk htl_stk mem mem' blk ge id,
+  Lemma mem_alloc_zero_match_frames : forall rtl_stk htl_stk mem mem' blk id,
       Mem.alloc mem 0 0 = (mem', blk) ->
-      match_frames ge id mem rtl_stk htl_stk ->
-      match_frames ge id mem' rtl_stk htl_stk.
+      match_frames prog id mem rtl_stk htl_stk ->
+      match_frames prog id mem' rtl_stk htl_stk.
   Proof.
     Lemma mem_alloc_zero_match_arrs : forall m f sp blk mem mem' asa,
       Mem.alloc mem 0 0 = (mem', blk) ->
@@ -958,7 +969,7 @@ Section CORRECTNESS.
 
   Lemma eval_cond_correct :
     forall stk f sp pc rs mid m res ml st asr asa e b f' s s' args i cond,
-      match_states ge (RTL.State stk f sp pc rs m) (HTL.State res mid ml st asr asa) ->
+      match_states prog (RTL.State stk f sp pc rs m) (HTL.State res mid ml st asr asa) ->
       (forall v, In v args -> Ple v (RTL.max_reg_function f)) ->
       Op.eval_condition cond (map (fun r : positive => Registers.Regmap.get r rs) args) m = Some b ->
       translate_condition cond args s = OK e s' i ->
@@ -1089,7 +1100,7 @@ Section CORRECTNESS.
 
   Lemma eval_cond_correct' :
     forall e stk f sp pc rs m res mid ml st asr asa v f' s s' args i cond,
-      match_states ge (RTL.State stk f sp pc rs m) (HTL.State res mid ml st asr asa) ->
+      match_states prog (RTL.State stk f sp pc rs m) (HTL.State res mid ml st asr asa) ->
       (forall v, In v args -> Ple v (RTL.max_reg_function f)) ->
       Values.Val.of_optbool None = v ->
       translate_condition cond args s = OK e s' i ->
@@ -1102,7 +1113,7 @@ Section CORRECTNESS.
 
   Lemma eval_correct_Oshrximm :
     forall s sp rs m v e asr asa f f' stk s' i pc res0 pc' args res mid ml st n,
-      match_states ge (RTL.State stk f sp pc rs m) (HTL.State res mid ml st asr asa) ->
+      match_states prog (RTL.State stk f sp pc rs m) (HTL.State res mid ml st asr asa) ->
       (RTL.fn_code f) ! pc = Some (RTL.Iop (Op.Oshrximm n) args res0 pc') ->
       Op.eval_operation ge sp (Op.Oshrximm n)
                         (List.map (fun r : BinNums.positive =>
@@ -1169,7 +1180,7 @@ Section CORRECTNESS.
 
   Lemma eval_correct :
     forall s sp op rs m v e asr asa f f' stk s' i pc res0 pc' args res mid ml st ,
-      match_states ge (RTL.State stk f sp pc rs m) (HTL.State res mid ml st asr asa) ->
+      match_states prog (RTL.State stk f sp pc rs m) (HTL.State res mid ml st asr asa) ->
       (RTL.fn_code f) ! pc = Some (RTL.Iop op args res0 pc') ->
       Op.eval_operation ge sp op
                         (List.map (fun r : BinNums.positive => Registers.Regmap.get r rs) args) m = Some v ->
@@ -1470,9 +1481,9 @@ Section CORRECTNESS.
       (rs : RTL.regset) (m : mem) (pc' : RTL.node),
       (RTL.fn_code f) ! pc = Some (RTL.Inop pc') ->
       forall R1 : HTL.state,
-        match_states ge (RTL.State s f sp pc rs m) R1 ->
+        match_states prog (RTL.State s f sp pc rs m) R1 ->
         exists R2 : HTL.state,
-          Smallstep.plus HTL.step tge R1 Events.E0 R2 /\ match_states ge (RTL.State s f sp pc' rs m) R2.
+          Smallstep.plus HTL.step tge R1 Events.E0 R2 /\ match_states prog (RTL.State s f sp pc' rs m) R2.
   Proof.
     intros * H R1 MSTATE.
     inv_state.
@@ -1510,10 +1521,10 @@ Section CORRECTNESS.
       (RTL.fn_code f) ! pc = Some (RTL.Iop op args res0 pc') ->
       Op.eval_operation ge sp op (map (fun r : positive => Registers.Regmap.get r rs) args) m = Some v ->
       forall R1 : HTL.state,
-        match_states ge (RTL.State s f sp pc rs m) R1 ->
+        match_states prog (RTL.State s f sp pc rs m) R1 ->
         exists R2 : HTL.state,
           Smallstep.plus HTL.step tge R1 Events.E0 R2 /\
-          match_states ge (RTL.State s f sp pc' (Registers.Regmap.set res0 v rs) m) R2.
+          match_states prog (RTL.State s f sp pc' (Registers.Regmap.set res0 v rs) m) R2.
   Proof.
     intros * H H0 R1 MSTATE.
     inv_state. inv MARR.
@@ -1687,10 +1698,10 @@ Section CORRECTNESS.
       (m : mem) (m' : Mem.mem') (stk : Values.block),
       Mem.alloc m 0 (RTL.fn_stacksize f) = (m', stk) ->
       forall R1 : HTL.state,
-        match_states ge (RTL.Callstate s (AST.Internal f) args m) R1 ->
+        match_states prog (RTL.Callstate s (AST.Internal f) args m) R1 ->
         exists R2 : HTL.state,
           Smallstep.plus HTL.step tge R1 Events.E0 R2 /\
-          match_states ge
+          match_states prog
             (RTL.State s f (Values.Vptr stk Integers.Ptrofs.zero) (RTL.fn_entrypoint f)
                        (RTL.init_regs args (RTL.fn_params f)) m') R2.
   Proof.
@@ -2099,10 +2110,10 @@ Section CORRECTNESS.
       (RTL.fn_code f) ! pc = Some (RTL.Icall sig fn args dst pc') ->
       RTL.find_function ge fn rs = Some fd ->
       forall R1 : HTL.state,
-        match_states ge (RTL.State s f sp pc rs m) R1 ->
+        match_states prog (RTL.State s f sp pc rs m) R1 ->
         exists R2 : HTL.state,
           Smallstep.plus HTL.step tge R1 Events.E0 R2 /\
-          match_states ge (RTL.Callstate (RTL.Stackframe dst f sp pc' rs :: s) fd
+          match_states prog (RTL.Callstate (RTL.Stackframe dst f sp pc' rs :: s) fd
                                          (List.map (fun r => Registers.Regmap.get r rs) args) m)
                        R2.
   Proof.
@@ -2296,10 +2307,10 @@ Section CORRECTNESS.
       (RTL.fn_code f) ! pc = Some (RTL.Ireturn or) ->
       Mem.free m stk 0 (RTL.fn_stacksize f) = Some m' ->
       forall R1 : HTL.state,
-        match_states ge (RTL.State s f (Values.Vptr stk Integers.Ptrofs.zero) pc rs m) R1 ->
+        match_states prog (RTL.State s f (Values.Vptr stk Integers.Ptrofs.zero) pc rs m) R1 ->
         exists R2 : HTL.state,
           Smallstep.plus HTL.step tge R1 Events.E0 R2 /\
-          match_states ge (RTL.Returnstate s (Registers.regmap_optget or Values.Vundef rs) m') R2.
+          match_states prog (RTL.Returnstate s (Registers.regmap_optget or Values.Vundef rs) m') R2.
   Proof.
     intros * H H0 * MSTATE.
     inv_state.
@@ -2343,10 +2354,10 @@ Section CORRECTNESS.
     forall (res0 : Registers.reg) (f : RTL.function) (sp : Values.val) (pc : RTL.node)
       (rs : RTL.regset) (s : list RTL.stackframe) (vres : Values.val) (m : mem)
       (R1 : HTL.state),
-      match_states ge (RTL.Returnstate (RTL.Stackframe res0 f sp pc rs :: s) vres m) R1 ->
+      match_states prog (RTL.Returnstate (RTL.Stackframe res0 f sp pc rs :: s) vres m) R1 ->
       exists R2 : HTL.state,
         Smallstep.plus HTL.step tge R1 Events.E0 R2 /\
-        match_states ge (RTL.State s f sp pc (Registers.Regmap.set res0 vres rs) m) R2.
+        match_states prog (RTL.State s f sp pc (Registers.Regmap.set res0 vres rs) m) R2.
   Proof.
     intros * MSTATE.
     inv MSTATE.
@@ -2535,10 +2546,10 @@ Section CORRECTNESS.
       Op.eval_addressing ge sp addr (map (fun r : positive => Registers.Regmap.get r rs) args) = Some a ->
       Mem.loadv chunk m a = Some v ->
       forall R1 : HTL.state,
-        match_states ge (RTL.State s f sp pc rs m) R1 ->
+        match_states prog (RTL.State s f sp pc rs m) R1 ->
         exists R2 : HTL.state,
           Smallstep.plus HTL.step tge R1 Events.E0 R2 /\
-          match_states ge (RTL.State s f sp pc' (Registers.Regmap.set dst v rs) m) R2.
+          match_states prog (RTL.State s f sp pc' (Registers.Regmap.set dst v rs) m) R2.
   Proof.
     intros s f sp pc rs m chunk addr args dst pc' a v H H0 H1 R1 MSTATE.
     inv_state.
@@ -2935,9 +2946,9 @@ Section CORRECTNESS.
       Op.eval_addressing ge sp addr (map (fun r : positive => Registers.Regmap.get r rs) args) = Some a ->
       Mem.storev chunk m a (Registers.Regmap.get src rs) = Some m' ->
       forall R1 : HTL.state,
-        match_states ge (RTL.State s f sp pc rs m) R1 ->
+        match_states prog (RTL.State s f sp pc rs m) R1 ->
         exists R2 : HTL.state,
-          Smallstep.plus HTL.step tge R1 Events.E0 R2 /\ match_states ge (RTL.State s f sp pc' rs m') R2.
+          Smallstep.plus HTL.step tge R1 Events.E0 R2 /\ match_states prog (RTL.State s f sp pc' rs m') R2.
   Proof.
     intros s f sp pc rs m chunk addr args src pc' a m' H H0 H1 R1 MSTATES.
     inv_state. inv_arr_access.
@@ -3806,9 +3817,9 @@ Section CORRECTNESS.
       Op.eval_condition cond (map (fun r : positive => Registers.Regmap.get r rs) args) m = Some b ->
       pc' = (if b then ifso else ifnot) ->
       forall R1 : HTL.state,
-        match_states ge (RTL.State s f sp pc rs m) R1 ->
+        match_states prog (RTL.State s f sp pc rs m) R1 ->
         exists R2 : HTL.state,
-          Smallstep.plus HTL.step tge R1 Events.E0 R2 /\ match_states ge (RTL.State s f sp pc' rs m) R2.
+          Smallstep.plus HTL.step tge R1 Events.E0 R2 /\ match_states prog (RTL.State s f sp pc' rs m) R2.
   Proof.
     intros s f sp pc rs m cond args ifso ifnot b pc' H H0 H1 R1 MSTATE.
     inv_state.
@@ -3865,9 +3876,9 @@ Section CORRECTNESS.
       Registers.Regmap.get arg rs = Values.Vint n ->
       list_nth_z tbl (Integers.Int.unsigned n) = Some pc' ->
       forall R1 : HTL.state,
-        match_states ge (RTL.State s f sp pc rs m) R1 ->
+        match_states prog (RTL.State s f sp pc rs m) R1 ->
         exists R2 : HTL.state,
-          Smallstep.plus HTL.step tge R1 Events.E0 R2 /\ match_states ge (RTL.State s f sp pc' rs m) R2.
+          Smallstep.plus HTL.step tge R1 Events.E0 R2 /\ match_states prog (RTL.State s f sp pc' rs m) R2.
   Proof.
     intros s f sp pc rs m arg tbl n pc' H H0 H1 R1 MSTATE.
   
@@ -3897,7 +3908,7 @@ Section CORRECTNESS.
     forall s1 : Smallstep.state (RTL.semantics prog),
       Smallstep.initial_state (RTL.semantics prog) s1 ->
       exists s2 : Smallstep.state (HTL.semantics tprog),
-        Smallstep.initial_state (HTL.semantics tprog) s2 /\ match_states ge s1 s2.
+        Smallstep.initial_state (HTL.semantics tprog) s2 /\ match_states prog s1 s2.
   Proof.
     induction 1.
     destruct TRANSL.
@@ -3938,7 +3949,7 @@ Section CORRECTNESS.
     forall (s1 : Smallstep.state (RTL.semantics prog))
            (s2 : Smallstep.state (HTL.semantics tprog))
            (r : Integers.Int.int),
-      match_states ge s1 s2 ->
+      match_states prog s1 s2 ->
       Smallstep.final_state (RTL.semantics prog) s1 r ->
       Smallstep.final_state (HTL.semantics tprog) s2 r.
   Proof.
@@ -3952,8 +3963,8 @@ Section CORRECTNESS.
     forall (S1 : RTL.state) t S2,
       RTL.step ge S1 t S2 ->
       forall (R1 : HTL.state),
-        match_states ge S1 R1 ->
-        exists R2, Smallstep.plus HTL.step tge R1 t R2 /\ match_states ge S2 R2.
+        match_states prog S1 R1 ->
+        exists R2, Smallstep.plus HTL.step tge R1 t R2 /\ match_states prog S2 R2.
   Proof.
     induction 1; eauto with htlproof; try solve [ intros; inv_state ].
   Qed.
